src/Model.QUIC.fsti
@@ -15,6 +15,7 @@ module PNE = Model.PNE
 module SPNE = Spec.Agile.Cipher
 module BF = LowParse.BitFields
 module U62 = QUIC.UInt62
+module Secret = QUIC.Secret.Int
 
 open FStar.UInt32
 open Mem
@@ -288,12 +289,12 @@ val coerce: k:unsafe_id -> u:info ->
     writer_ae_info w == u1 /\
     writer_pne_info w == u2 /\
     writer_info w == u /\
-    writer_static_iv w ==
+    Model.Helpers.hide #12 (writer_static_iv w) ==
       Spec.derive_secret u1.AEAD.halg ts
         Spec.label_iv 12 /\
-    k1 == Spec.derive_secret u1.AEAD.halg ts
+    Model.Helpers.hide #(SAE.key_length u1.AEAD.alg) k1 == Spec.derive_secret u1.AEAD.halg ts
         Spec.label_key (SAE.key_length u1.AEAD.alg) /\
-    k2 == QUIC.Spec.derive_secret u2.PNE.halg ts
+    Model.Helpers.hide #(PNE.key_len u2) k2 == QUIC.Spec.derive_secret u2.PNE.halg ts
         QUIC.Spec.label_hp (PNE.key_len u2)
   )
 
@@ -346,7 +347,7 @@ val encrypt
     (if Spec.is_retry h then l = 0
     else (
       Spec.has_payload_length h ==>
-        U64.v (Spec.payload_length h) == l
+        Secret.v (Spec.payload_length h) == l
 	  + Spec.Agile.AEAD.tag_length (writer_ae_info w).AEAD.alg))
   )
   (ensures fun h0 c h1 ->
@@ -361,7 +362,7 @@ val encrypt
       (let ea = (writer_ae_info w).AE.alg in
       let k1, k2 = writer_leak w in
       let plain : Spec.pbytes = (writer_info w).plain_pkg.repr p in
-      c == Spec.encrypt ea k1 (writer_static_iv w) k2 h
+      c == Spec.encrypt ea (Model.Helpers.hide #(Seq.length k1) k1) (Model.Helpers.hide #12 (writer_static_iv w)) (Model.Helpers.hide #(Seq.length k2) k2) h
 	(plain <: Spec.pbytes' (Spec.is_retry h)))
     ))
 
@@ -425,7 +426,7 @@ val decrypt
     (match res with
     | M_Failure -> expected_pnT r h1 == expected
     | M_Success h _ _ _ ->
-      expected_pnT r h1 == max62 (Spec.packet_number h) expected) /\
+      expected_pnT r h1 == max62 (Secret.reveal (Spec.packet_number h)) expected) /\
     (safe k ==> (
       match get_sample packet cid_len with
       | _ -> True
@@ -433,7 +434,7 @@ val decrypt
     (unsafe k ==>
       (let ea = (writer_ae_info w).AE.alg in
       let k1, k2 = reader_leak r in
-      match Spec.decrypt ea k1 (writer_static_iv w) k2
+      match Spec.decrypt ea (Model.Helpers.hide #(Seq.length k1) k1) (Model.Helpers.hide #12 (writer_static_iv w)) (Model.Helpers.hide #(Seq.length k2) k2)
 	    (UInt64.v expected) cid_len packet,
 	    res
       with
